@prefix dc:           <http://purl.org/dc/elements/1.1/> .
@prefix dcterms:      <http://purl.org/dc/terms/> .
@prefix geo:          <http://www.opengis.net/ont/geosparql#> .
@prefix gwml2:        <http://gwml2.org/def/gwml2#> .
@prefix hyf:          <https://www.opengis.net/def/schema/hy_features/hyf/> .
@prefix hyfo:         <http://hyfo.spatialai.org/v1/hyfo#> .
@prefix kwg-ont:      <http://stko-kwg.geog.ucsb.edu/lod/ontology/> .
@prefix nhdplusv2:    <http://nhdplusv2.spatialai.org/v1/nhdplusv2#> .
@prefix owl:          <http://www.w3.org/2002/07/owl#> .
@prefix quantitykind: <http://qudt.org/vocab/quantitykind/> .
@prefix qudt:         <http://qudt.org/schema/qudt/> .
@prefix rdf:          <http://www.w3.org/1999/02/22-rdf-syntax-ns#> .
@prefix rdfs:         <http://www.w3.org/2000/01/rdf-schema#> .
@prefix schema:       <https://schema.org/> .
@prefix skos:         <http://www.w3.org/2004/02/skos/core#> .
@prefix spatial:      <http://purl.org/spatialai/spatial/spatial-full#> .
@prefix unit:         <http://qudt.org/vocab/unit/> .
@prefix wdt:          <https://www.wikidata.org/prop/direct/> .
@prefix xml:          <http://www.w3.org/XML/1998/namespace> .
@prefix xsd:          <http://www.w3.org/2001/XMLSchema#> .

<http://purl.org/spatialai/spatial/water-full> rdf:type owl:Ontology ;
                                               dcterms:creator <https://orcid.org/0000-0002-9070-3169> ; # David Kedrowski
                                               dcterms:created "2024-09-04"^^xsd:date ;
                                               dcterms:contributor <https://orcid.org/0000-0002-5331-5052> , # Torsten Hahmann
																   <https://orcid.org/0000-0002-9070-3169> , # David Kedrowski
																   <https://orcid.org/0000-0003-3271-6700> ; # Katrina Schweikert
                                               dcterms:modified "2025-04-21"^^xsd:date ;
                                               dcterms:publisher <https://sawgraph.github.io/> ;
											   dcterms:issued "2025-04-21"^^xsd:date ;
											   dc:source <https://raw.githubusercontent.com/SAWGraph/water-kg/refs/heads/main/ontologies/sawgraph-water-ontology.ttl> ;
                                               dcterms:description "This ontology supports querying the SAWGraph Knowledge Graph. It adapts and extends concepts from HY_Features, HyFO, and GWML2"@en ;
                                               dcterms:title "SAWGraph's hydrology (water) ontology - an adaptation and extension of concepts from HY_Features, HyFO, and GWML2"@en ;
											   rdfs:label "SAWGraph's hydrology (water) ontology - an adaptation and extension of concepts from HY_Features, HyFO, and GWML2"@en ;
                                               owl:versionInfo "1.0"@en .

#################################################################
#    Annotation properties
#################################################################

###  http://purl.org/dc/terms/contributor
dcterms:contributor rdf:type owl:AnnotationProperty .

###  http://purl.org/dc/terms/created
dcterms:created rdf:type owl:AnnotationProperty .

###  http://purl.org/dc/terms/modified
dcterms:modified rdf:type owl:AnnotationProperty .

###  http://purl.org/dc/terms/creator
dcterms:creator rdf:type owl:AnnotationProperty .

###  http://purl.org/dc/terms/publisher
dcterms:publisher rdf:type owl:AnnotationProperty .

###  http://purl.org/dc/terms/description
dcterms:description rdf:type owl:AnnotationProperty .

###  http://purl.org/dc/terms/title
dcterms:title rdf:type owl:AnnotationProperty .

###  http://www.w3.org/2004/02/skos/core#definition
skos:definition rdf:type owl:AnnotationProperty .

###  http://www.w3.org/2004/02/skos/core#description
skos:description rdf:type owl:AnnotationProperty .

###  http://www.w3.org/2004/02/skos/core#editorialNote
skos:editorialNote rdf:type owl:AnnotationProperty .

###  http://www.w3.org/2004/02/skos/core#example
skos:example rdf:type owl:AnnotationProperty .

###  http://www.w3.org/2004/02/skos/core#note
skos:note rdf:type owl:AnnotationProperty .

###  http://www.w3.org/2004/02/skos/core#prefLabel
skos:prefLabel rdf:type owl:AnnotationProperty .

###  https://schema.org/name
schema:name rdf:type rdf:Property ;
			rdfs:subPropertyOf rdfs:label ;
			owl:equivalentProperty dcterms:title ;
			schema:domainIncludes schema:Thing ;
			schema:rangeIncludes schema:Text ;
			rdfs:label "schema:name"^^xsd:string ;
			rdfs:comment "The name of the item."^^xsd:string .

#################################################################
#    Datatypes
#################################################################




#################################################################
#    Object Properties
#################################################################

### GeoSPARQL ###

###  http://www.opengis.net/ont/geosparql#defaultGeometry
geo:defaultGeometry rdf:type owl:ObjectProperty ;
                    rdfs:subPropertyOf geo:hasGeometry ;
	                rdfs:domain geo:Feature ;
	                rdfs:range geo:Geometry ;
					rdfs:label "geo:defaultGeometry"^^xsd:string ;
					rdfs:comment "The default Geometry to be used in spatial calculations. It is usually the most detailed Geometry."^^xsd:string ;
					rdfs:isDefinedBy geo: ,
		                             <http://www.opengis.net/spec/geosparql/1.1/req/geometry-extension/feature-properties> .

###  http://www.opengis.net/ont/geosparql#hasGeometry
geo:hasGeometry rdf:type owl:ObjectProperty ;
	            rdfs:domain geo:Feature ;
	            rdfs:range geo:Geometry ;
				rdfs:label "geo:hasGeometry"^^xsd:string ;
				rdfs:comment "A spatial representation for a given Feature."^^xsd:string ;
				rdfs:isDefinedBy geo: ,
		                         <http://www.opengis.net/spec/geosparql/1.0/req/geometry-extension/feature-properties> ,
		                         <http://www.opengis.net/spec/geosparql/1.1/req/geometry-extension/feature-properties> .

### Groundwater Markup Language v2.2 ###

###  http://gwml2.org/def/gwml2#gwAquiferSystem
gwml2:gwAquiferSystem rdf:type owl:ObjectProperty ;
                      rdfs:domain gwml2:GW_Aquifer ;
					  rdfs:range gwml2:GW_AquiferSystem ;
				      rdfs:label "gwml2:gwAquiferSystem"^^xsd:string ;
				      rdfs:comment "Relates an aquifer system part, which can be another system, aquifer or confining bed, with its aquifer system"^^xsd:string ;
					  rdfs:isDefinedBy <https://docs.ogc.org/is/19-013/19-013.html> .

###  http://gwml2.org/def/gwml2#gwAquiferSystemPart
gwml2:gwAquiferSystemPart rdf:type owl:ObjectProperty ;
                          owl:inverseOf gwml2:gwAquiferSystem ;
				          rdfs:label "gwml2:gwAquiferSystemPart"^^xsd:string ;
				          rdfs:comment "Relates an aquifer system with its parts, which can be other systems, aquifers or confining beds"^^xsd:string ;
						  rdfs:isDefinedBy <https://docs.ogc.org/is/19-013/19-013.html> .

###  http://gwml2.org/def/gwml2#gwMonitoringHost
gwml2:gwMonitoringHost rdf:type owl:ObjectProperty ;
                       rdfs:domain gwml2:GW_MonitoringSite ;
					   rdfs:range hyfo:WaterFeature ;
					   rdfs:label "gwml2:gwMonitoringHost"^^xsd:string ;
					   rdfs:comment "Identifies the feature hosting the site [GW_MonitoringSite], e.g., a well, spring, lake or stream"^^xsd:string ;
					   rdfs:isDefinedBy <https://docs.ogc.org/is/19-013/19-013.html> .

###  http://gwml2.org/def/gwml2#gwWellUnit
gwml2:gwWellUnit rdf:type owl:ObjectProperty ;
                 owl:equivalentProperty hyfo:tapsAquifer ;
				 rdfs:domain gwml2:GW_Well ;
				 rdfs:range gwml2:GW_AquiferUnit ;
				 rdfs:label "gwml2:gwWellUnit"^^xsd:string ;
				 rdfs:comment "Identifies the aquifers or confining beds intersecting the well"^^xsd:string ;
				 rdfs:isDefinedBy <https://docs.ogc.org/is/19-013/19-013.html> .

### HY_Features ###

###  https://www.opengis.net/def/schema/hy_features/hyf/downstreamWaterBody
hyf:downstreamWaterBody rdf:type owl:ObjectProperty ;
						rdfs:subPropertyOf nhdplusv2:downstreamWaterBodyTC ;
						owl:inverseOf hyf:upstreamWaterBody ;
				        rdfs:label "hyf:downstreamWaterBody"^^xsd:string ;
				        rdfs:comment "Identifies another waterbody immediately downstream, allowing network navigation without knowing an inflow or outflow of the catchment realized by the waterbody"^^xsd:string ;
						rdfs:isDefinedBy <https://docs.ogc.org/is/14-111r6/14-111r6.html> ,
						                 <https://github.com/opengeospatial/HY_Features/tree/master/ontology> .

###  https://www.opengis.net/def/schema/hy_features/hyf/realizedCatchment
hyf:realizedCatchment rdf:type owl:ObjectProperty ;
					  rdfs:domain hyf:HY_CatchmentRealization ;
					  rdfs:range hyf:HY_Catchment ;
				      rdfs:label "hyf:realizedCatchment"^^xsd:string ;
				      rdfs:comment "Identifies the one and only one catchment that is realized by a particular feature"^^xsd:string ;
					  rdfs:isDefinedBy <https://docs.ogc.org/is/14-111r6/14-111r6.html> ,
						               <https://github.com/opengeospatial/HY_Features/tree/master/ontology> .

###  https://www.opengis.net/def/schema/hy_features/hyf/upstreamWaterBody
hyf:upstreamWaterBody rdf:type owl:ObjectProperty ;
					  owl:inverseOf hyf:downstreamWaterBody ;
				      rdfs:label "hyf:upstreamWaterBody"^^xsd:string ;
				      rdfs:comment "Identifies another waterbody immediately upstream, allowing network navigation without knowing an inflow or outflow of the catchment realized by the waterbody"^^xsd:string ;
					  rdfs:isDefinedBy <https://docs.ogc.org/is/14-111r6/14-111r6.html> ,
						               <https://github.com/opengeospatial/HY_Features/tree/master/ontology> .

### HY_Features (SAWGraph extension) ###

###  http://nhdplusv2.spatialai.org/v1/nhdplusv2#downstreamWaterBodyTC
nhdplusv2:downstreamWaterBodyTC rdf:type owl:ObjectProperty ,
								         owl:TransitiveProperty ;
						        rdfs:domain _:UnionHydrofeatureWaterfeaturerealization ;
						        rdfs:range _:UnionHydrofeatureWaterfeaturerealization ;
				                rdfs:label "nhdplusv2:downstreamWaterBodyTC"^^xsd:string ;
				                rdfs:comment "The transitive closure of the nhdplusv2:downstreamWaterBody object property"^^xsd:string .

_:UnionHydrofeatureWaterfeaturerealization rdf:type owl:Class ;
                                           owl:unionOf ( hyf:HY_HydroFeature hyfo:WaterFeatureRepresentation ) .

###  http://nhdplusv2.spatialai.org/v1/nhdplusv2#downstreamFlowPath
nhdplusv2:downstreamFlowPath rdf:type owl:ObjectProperty ;
					         rdfs:subPropertyOf nhdplusv2:downstreamFlowPathTC ,
					                            hyf:downstreamWaterBody ;
					         owl:inverseOf nhdplusv2:upstreamFlowPath ;
				             rdfs:label "nhdplusv2:downstreamFlowPath"^^xsd:string ;
				             rdfs:comment "Identifies another flowpath immediately downstream, allowing network navigation without knowing an inflow or outflow of the catchment realized by the flowpath"^^xsd:string .

###  http://nhdplusv2.spatialai.org/v1/nhdplusv2#downstreamFlowPathTC
nhdplusv2:downstreamFlowPathTC rdf:type owl:ObjectProperty ,
								        owl:TransitiveProperty ;
						       rdfs:subPropertyOf nhdplusv2:downstreamWaterBodyTC ;
						       rdfs:domain hyf:HY_FlowPath ;
						       rdfs:range hyf:HY_FlowPath ;
				               rdfs:label "nhdplusv2:downstreamFlowPathTC"^^xsd:string ;
				               rdfs:comment "The transitive closure of the nhdplusv2:downstreamFlowPath object property"^^xsd:string .

###  http://nhdplusv2.spatialai.org/v1/nhdplusv2#upstreamFlowPath
nhdplusv2:upstreamFlowPath rdf:type owl:ObjectProperty ;
                           rdfs:subPropertyOf hyf:upstreamWaterBody ;
					       owl:inverseOf nhdplusv2:downstreamFlowPath ;
				           rdfs:label "nhdplusv2:upstreamFlowPath"^^xsd:string ;
				           rdfs:comment "Identifies another flowpath immediately upstream, allowing network navigation without knowing an inflow or outflow of the catchment realized by the flowpath"^^xsd:string .

###  http://nhdplusv2.spatialai.org/v1/nhdplusv2#partOfFlowPath
nhdplusv2:partOfFlowPath rdf:type owl:ObjectProperty ;
				         rdfs:domain nhdplusv2:FlowLine ;
				         rdfs:range nhdplusv2:FlowPath ;
				         rdfs:label "nhdplusv2:partOfFlowPath"^^xsd:string ;
				         rdfs:comment "Connects an elementary flowpath (e.g., NHDFlowline) to any non-elementary flowpath it is a part of"^^xsd:string .

###  http://nhdplusv2.spatialai.org/v1/nhdplusv2#associatedCatchmentArea
nhdplusv2:associatedCatchmentArea rdf:type owl:ObjectProperty ;
					              rdfs:domain nhdplusv2:FlowPath ;
					              rdfs:range hyf:HY_CatchmentArea ;
				                  rdfs:label "nhdplusv2:associatedCatchmentArea"^^xsd:string ;
				                  rdfs:comment "Identifies the one and only one catchment area that is associated with a particular flowpath"^^xsd:string .

### Hydro Foundational Ontology ###

###  http://hyfo.spatialai.org/v1/hyfo#isRepresentedByWFR
hyfo:isRepresentedByWFR rdf:type owl:ObjectProperty ;
					    rdfs:domain hyfo:WaterFeature ;
					    rdfs:range hyfo:WaterFeatureRepresentation ;
				        rdfs:label "hyfo:isRepresentedByWFR"^^xsd:string ;
				        rdfs:comment "Relates a water feature to a representation of that water feature"^^xsd:string .

### NHDPlus V2 ###

###  http://nhdplusv2.spatialai.org/v1/nhdplusv2#hasFlowPathLength
nhdplusv2:hasFlowPathLength rdf:type owl:ObjectProperty ;
				            rdfs:range qudt:Quantity ;
				            rdfs:label "nhdplusv2:hasFlowPathLength"^^xsd:string ;
				            rdfs:comment "Relates any flowpath to its length, represented as, for example, a qudt:Quantity object"^^xsd:string .

### QUDT ###

###  http://qudt.org/schema/qudt/quantityValue
qudt:quantityValue rdf:type owl:ObjectProperty ;
				   rdfs:range qudt:QuantityValue ;
				   rdfs:label "qudt:quantityValue"^^xsd:string ;
				   rdfs:isDefinedBy <http://qudt.org/2.1/schema/qudt> .

###  http://qudt.org/schema/qudt/hasUnit
qudt:hasUnit rdf:type owl:ObjectProperty ;
			 rdfs:label "qudt:hasUnit"^^xsd:string ;
			 rdfs:isDefinedBy <http://qudt.org/2.1/schema/qudt> .

###  http://qudt.org/schema/qudt/hasQuantityKind
qudt:hasQuantityKind rdf:type owl:ObjectProperty ;
					 rdfs:range qudt:QuantityKind ;
					 rdfs:label "qudt:hasQuantityKind"^^xsd:string ;
					 rdfs:isDefinedBy <http://qudt.org/2.1/schema/qudt> .

### SAWGraph Spatial Ontology ###

###  http://purl.org/spatialai/spatial/spatial-full#connectedTo
spatial:connectedTo rdf:type owl:ObjectProperty ;
                    rdfs:subPropertyOf spatial:spatiallyRelatedTo ;
                    rdfs:label "spatial:connectedTo"^^xsd:string ;
					rdfs:comment "topological connection (spatial contact) (sawgraph)" .


#################################################################
#    Datatype Properties
#################################################################

### NHDPlus V2 ###

###  http://nhdplusv2.spatialai.org/v1/nhdplusv2#hasCOMID
nhdplusv2:hasCOMID rdf:type owl:DatatypeProperty ;
				   rdfs:label "nhdplusv2:hasCOMID"^^xsd:string ;
				   rdfs:comment "Relates an NHDPlusV2 feature to its COMID"^^xsd:string .

###  http://nhdplusv2.spatialai.org/v1/nhdplusv2#hasFCODE
nhdplusv2:hasFCODE rdf:type owl:DatatypeProperty ;
				   rdfs:label "nhdplusv2:hasFCODE"^^xsd:string ;
				   rdfs:comment "Relates an NHDPlusV2 feature to its FCODE (see also nhdplusv2:hasFTYPE)"^^xsd:string .

###  http://nhdplusv2.spatialai.org/v1/nhdplusv2#hasFTYPE
nhdplusv2:hasFTYPE rdf:type owl:DatatypeProperty ;
				   rdfs:label "nhdplusv2:hasFTYPE"^^xsd:string ;
				   rdfs:comment "Relates an NHDPlusV2 feature to its FTYPE (see also nhdplusv2:hasFCODE)"^^xsd:string .

###  http://nhdplusv2.spatialai.org/v1/nhdplusv2#hasReachCode
nhdplusv2:hasReachCode rdf:type owl:DatatypeProperty ;
				       rdfs:label "nhdplusv2:hasReachCode"^^xsd:string ;
				       rdfs:comment "Relates an NHDPlusV2 feature to its ReachCode"^^xsd:string .

### QUDT ###

###  http://qudt.org/schema/qudt/numericValue
qudt:numericValue rdf:type owl:DatatypeProperty ;
				  rdfs:range qudt:NumericUnion ;
				  rdfs:label "qudt:numericValue"^^xsd:string ;
				  rdfs:isDefinedBy <http://qudt.org/2.1/schema/qudt> .

#################################################################
#    Classes
#################################################################

### GeoSPARQL ###

###  http://www.opengis.net/ont/geosparql#Feature
geo:Feature rdf:type owl:Class ;
            rdfs:subClassOf geo:SpatialObject ;
			owl:disjointWith geo:Geometry  ;
            rdfs:label "geo:Feature"^^xsd:string ;
            rdfs:comment "A discrete spatial phenomenon in a universe of discourse."^^xsd:string ;
			rdfs:isDefinedBy geo: ,
		                     <http://www.opengis.net/spec/geosparql/1.0/req/core/feature-class> ,
		                     <http://www.opengis.net/spec/geosparql/1.1/req/core/feature-class> . 

###  http://www.opengis.net/ont/geosparql#Geometry
geo:Geometry rdf:type owl:Class ;
             rdfs:subClassOf geo:SpatialObject ;
             rdfs:label "geo:Geometry"^^xsd:string ;
             rdfs:comment "A coherent set of direct positions in space. The positions are held within a Spatial Reference System (SRS)."^^xsd:string ;
			 rdfs:isDefinedBy geo: ,
		                      <http://www.opengis.net/spec/geosparql/1.0/req/geometry-extension/geometry-class> ,
		                      <http://www.opengis.net/spec/geosparql/1.1/req/geometry-extension/geometry-class> .

###  http://www.opengis.net/ont/geosparql#SpatialObject
geo:SpatialObject rdf:type owl:Class ;
                  rdfs:label "geo:SpatialObject"^^xsd:string ;
                  rdfs:comment "Anything spatial (being or having a shape, position or an extent)."^^xsd:string ;
				  rdfs:isDefinedBy geo: ,
		                           <http://www.opengis.net/spec/geosparql/1.0/req/core/spatial-object-class> ,
		                           <http://www.opengis.net/spec/geosparql/1.1/req/core/spatial-object-class> .

### Groundwater Markup Language v2.2 ###

###  http://gwml2.org/def/gwml2#GW_Aquifer
gwml2:GW_Aquifer rdf:type owl:Class ;
                 rdfs:subClassOf gwml2:GW_AquiferUnit ;
				 rdfs:label "gwml2:GW_Aquifer"^^xsd:string ;
				 rdfs:comment "A body of earth material that contains / potentially contains / potentially contained sufficient saturated permeable material to yield significant quantities of water to wells and springs (after Lohman, 1972)"^^xsd:string ;
				 rdfs:isDefinedBy <https://docs.ogc.org/is/19-013/19-013.html> .

###  http://gwml2.org/def/gwml2#GW_AquiferSystem
gwml2:GW_AquiferSystem rdf:type owl:Class ;
                       rdfs:subClassOf gwml2:GW_AquiferUnit ;
				       rdfs:label "gwml2:GW_AquiferSystem"^^xsd:string ;
				       rdfs:comment "A body of permeable and poorly permeable material that functions regionally as a water-yielding unit; it comprises two or more permeable beds separated at least locally by confining beds that impede groundwater movement but do not greatly affect the regional hydraulic continuity of the system; includes both saturated and unsaturated parts of permeable material (after ASCE, 1987)"^^xsd:string ;
					   rdfs:isDefinedBy <https://docs.ogc.org/is/19-013/19-013.html> .

###  http://gwml2.org/def/gwml2#GW_AquiferUnit
gwml2:GW_AquiferUnit rdf:type owl:Class ;
                     rdfs:subClassOf gwml2:GW_HydrogeoUnit ,
					                 hyfo:AquiferWaterFeature ;
				     rdfs:label "gwml2:GW_AquiferUnit"^^xsd:string ;
				     rdfs:comment "Denotes aquifer-related hydrogeological units: aquifer systems, aquifers, or confining beds"^^xsd:string ;
					 rdfs:isDefinedBy <https://docs.ogc.org/is/19-013/19-013.html> .

###  http://gwml2.org/def/gwml2#GW_HydrogeoUnit
gwml2:GW_HydrogeoUnit rdf:type owl:Class ;
				      rdfs:label "gwml2:GW_HydrogeoUnit"^^xsd:string ;
				      rdfs:comment "Any soil or rock unit or zone that by virtue of its hydraulic properties has a distinct influence on the storage or movement of groundwater (after ANS, 1980)"^^xsd:string ;
					  rdfs:isDefinedBy <https://docs.ogc.org/is/19-013/19-013.html> .

###  http://gwml2.org/def/gwml2#GW_MonitoringSite
gwml2:GW_MonitoringSite rdf:type owl:Class ;
				        rdfs:label "gwml2:GW_MonitoringSite"^^xsd:string ;
				        rdfs:comment "Site of observation related to groundwater"^^xsd:string ;
						rdfs:isDefinedBy <https://docs.ogc.org/is/19-013/19-013.html> .

###  http://gwml2.org/def/gwml2#GW_Well
gwml2:GW_Well rdf:type owl:Class ;
              rdfs:subClassOf hyfo:SubsurfaceWaterFeature ;
			  owl:equivalentClass hyfo:WaterWell ;
			  rdfs:label "gwml2:GW_Well"^^xsd:string ;
			  rdfs:comment "A shaft or hole sunk, dug or drilled into the Earth to observe, extract or inject water (after IGH1397)"^^xsd:string ;
			  rdfs:isDefinedBy <https://docs.ogc.org/is/19-013/19-013.html> .

### HY_Features ###

###  https://www.opengis.net/def/schema/hy_features/hyf/HY_Canal
hyf:HY_Canal rdf:type owl:Class ;
			 rdfs:subClassOf hyf:HY_WaterBody ;
			 rdfs:label "hyf:HY_Canal"^^xsd:string ;
			 rdfs:comment "a body of surface water, participating in a hydrographic network, that is special due to its artificial origin (man-made)"^^xsd:string ;
			 rdfs:isDefinedBy <https://docs.ogc.org/is/14-111r6/14-111r6.html> ,
						      <https://github.com/opengeospatial/HY_Features/tree/master/ontology> .

###  https://www.opengis.net/def/schema/hy_features/hyf/HY_Catchment
hyf:HY_Catchment rdf:type owl:Class ;
				 rdfs:subClassOf hyf:HY_HydroFeature ;
				 rdfs:label "hyf:HY_Catchment"^^xsd:string ;
				 rdfs:comment "captures the union of catchment and hydro nexus, and the multiple realizations of the holistic catchment concept"^^xsd:string ;
				 rdfs:isDefinedBy <https://docs.ogc.org/is/14-111r6/14-111r6.html> ,
						          <https://github.com/opengeospatial/HY_Features/tree/master/ontology> .

###  https://www.opengis.net/def/schema/hy_features/hyf/HY_CatchmentArea
hyf:HY_CatchmentArea rdf:type owl:Class ;
                     rdfs:subClassOf hyf:HY_CatchmentRealization ;
				     rdfs:label "hyf:HY_CatchmentArea"^^xsd:string ;
				     rdfs:comment "Two-dimensional (areal) hydrology-specific realization of the holistic catchment"^^xsd:string ;
					 rdfs:isDefinedBy <https://docs.ogc.org/is/14-111r6/14-111r6.html> ,
						              <https://github.com/opengeospatial/HY_Features/tree/master/ontology> .

###  https://www.opengis.net/def/schema/hy_features/hyf/HY_CatchmentDivide
hyf:HY_CatchmentDivide rdf:type owl:Class ;
                       rdfs:subClassOf hyf:HY_CatchmentRealization ;
				       rdfs:label "hyf:HY_CatchmentDivide"^^xsd:string ;
				       rdfs:comment "One-dimensional (linear) feature that is a hydrology-specific realization of the holistic catchment"^^xsd:string ;
					   rdfs:isDefinedBy <https://docs.ogc.org/is/14-111r6/14-111r6.html> ,
						                <https://github.com/opengeospatial/HY_Features/tree/master/ontology> .

###  https://www.opengis.net/def/schema/hy_features/hyf/HY_CatchmentRealization
hyf:HY_CatchmentRealization rdf:type owl:Class ;
                            rdfs:subClassOf hyfo:WaterFeatureRepresentation ;
				            rdfs:label "hyf:HY_CatchmentRealization"^^xsd:string ;
				            rdfs:comment "based on the idea that there are multiple hydrology-specific perspectives of the holistic catchment concept that are used to describe a catchment as a unit of study shared across sub-domains and studies"^^xsd:string ;
							rdfs:isDefinedBy <https://docs.ogc.org/is/14-111r6/14-111r6.html> ,
						                     <https://github.com/opengeospatial/HY_Features/tree/master/ontology> .

###  https://www.opengis.net/def/schema/hy_features/hyf/HY_Estuary
hyf:HY_Estuary rdf:type owl:Class ;
			   rdfs:subClassOf hyf:HY_WaterBody ;
			   rdfs:label "hyf:HY_Estuary"^^xsd:string ;
			   rdfs:comment "a body of surface water, participating in a hydrographic network, made special due to branching and its interaction with the open sea"^^xsd:string ;
			   rdfs:isDefinedBy <https://docs.ogc.org/is/14-111r6/14-111r6.html> ,
						        <https://github.com/opengeospatial/HY_Features/tree/master/ontology> .

###  https://www.opengis.net/def/schema/hy_features/hyf/HY_FlowPath
hyf:HY_FlowPath rdf:type owl:Class ;
				rdfs:subClassOf hyf:HY_CatchmentRealization ;
				rdfs:label "hyf:HY_FlowPath"^^xsd:string ;
				rdfs:comment "realizes a catchment specifically as a path connecting the inflow and outflow of the catchment it realizes"^^xsd:string ;
				rdfs:isDefinedBy <https://docs.ogc.org/is/14-111r6/14-111r6.html> ,
						         <https://github.com/opengeospatial/HY_Features/tree/master/ontology> .

###  https://www.opengis.net/def/schema/hy_features/hyf/HY_HydroFeature
hyf:HY_HydroFeature rdf:type owl:Class ;
                    rdfs:subClassOf geo:Feature ;
				    rdfs:label "hyf:HY_HydroFeature"^^xsd:string ;
				    rdfs:comment "a basic feature to reflect the properties that all hydrologic features have"^^xsd:string ;
					rdfs:isDefinedBy <https://docs.ogc.org/is/14-111r6/14-111r6.html> ,
						             <https://github.com/opengeospatial/HY_Features/tree/master/ontology> .

###  https://www.opengis.net/def/schema/hy_features/hyf/HY_Impoundment
hyf:HY_Impoundment rdf:type owl:Class ;
				   rdfs:subClassOf hyf:HY_WaterBody ;
				   rdfs:label "hyf:HY_Impoundment"^^xsd:string ;
				   rdfs:comment "a body of surface water, participating in a hydrographic network, seen as being special due to being formed by collecting water, for example in the case of a dam"^^xsd:string ;
				   rdfs:isDefinedBy <https://docs.ogc.org/is/14-111r6/14-111r6.html> ,
						            <https://github.com/opengeospatial/HY_Features/tree/master/ontology> .

###  https://www.opengis.net/def/schema/hy_features/hyf/HY_Lagoon
hyf:HY_Lagoon rdf:type owl:Class ;
			  rdfs:subClassOf hyf:HY_WaterBody ;
			  rdfs:label "hyf:HY_Lagoon"^^xsd:string ;
			  rdfs:comment "a body of surface water, participating in a hydrographic network, which is special due to its shallow depth and interaction with the open sea"^^xsd:string ;
			  rdfs:isDefinedBy <https://docs.ogc.org/is/14-111r6/14-111r6.html> ,
						       <https://github.com/opengeospatial/HY_Features/tree/master/ontology> .

###  https://www.opengis.net/def/schema/hy_features/hyf/HY_Lake
hyf:HY_Lake rdf:type owl:Class ;
			rdfs:subClassOf hyf:HY_WaterBody ;
			rdfs:label "hyf:HY_Lake"^^xsd:string ;
			rdfs:comment "a body of surface water, participating in a hydrographic network, made special due to its considerable size"^^xsd:string ;
			rdfs:isDefinedBy <https://docs.ogc.org/is/14-111r6/14-111r6.html> ,
						     <https://github.com/opengeospatial/HY_Features/tree/master/ontology> .

###  https://www.opengis.net/def/schema/hy_features/hyf/HY_River
hyf:HY_River rdf:type owl:Class ;
			 rdfs:subClassOf hyf:HY_WaterBody ;
		     rdfs:label "hyf:HY_River"^^xsd:string ;
			 rdfs:comment "a body of surface water, participating in a hydrographic network, which is special due to its property to permanently or temporarily flow"^^xsd:string ;
			 rdfs:isDefinedBy <https://docs.ogc.org/is/14-111r6/14-111r6.html> ,
						      <https://github.com/opengeospatial/HY_Features/tree/master/ontology> .

###  https://www.opengis.net/def/schema/hy_features/hyf/HY_WaterBody
hyf:HY_WaterBody rdf:type owl:Class ;
				 rdfs:subClassOf hyf:HY_HydroFeature ;
				 rdfs:subClassOf hyfo:SurfaceWaterFeature ;
				 rdfs:label "hyf:HY_WaterBody"^^xsd:string ;
				 rdfs:comment "A waterbody is part of the hydrographic network and is either standing in a depression or flowing in a channel, which are parts of the channel network"^^xsd:string ;
				 rdfs:isDefinedBy <https://docs.ogc.org/is/14-111r6/14-111r6.html> ,
						          <https://github.com/opengeospatial/HY_Features/tree/master/ontology> .

### NHDPlus V2 ###

###  https://nhdplusv2.spatialai.org/v1/nhdplusv2#FlowLine
nhdplusv2:FlowLine rdf:type owl:Class ;
				   rdfs:subClassOf nhdplusv2:FlowPath ;
				   rdfs:label "nhdplusv2:FlowLine"^^xsd:string ;
				   rdfs:comment "any atomic/elementary kind of HY_FlowPath within a given framework/context (for example, a single NHDFlowline instance)"^^xsd:string ;
				   rdfs:comment "area of associated catchment may be zero (per hydrologic fabric logic model)"^^xsd:string ;
				   rdfs:comment "can be part of at most one mainstem"^^xsd:string ;
				   rdfs:subClassOf [ rdf:type owl:Restriction ;
				                     owl:onProperty nhdplusv2:partOfFlowPath ;
								     owl:maxQualifiedCardinality "1"^^xsd:nonNegativeInteger;
								     owl:onClass nhdplusv2:MainStem
								   ] .

###  https://nhdplusv2.spatialai.org/v1/nhdplusv2#FlowPath
nhdplusv2:FlowPath rdf:type owl:Class ;
			       rdfs:subClassOf hyf:HY_FlowPath ;
			       rdfs:label "nhdplusv2:FlowPath"^^xsd:string ;
			       rdfs:comment "any non-atomic/non-elementary kind of HY_FlowPath comprised of a contiguous set of atomic/elementary flowpaths"^^xsd:string .

###  https://nhdplusv2.spatialai.org/v1/nhdplusv2#MainStem
nhdplusv2:MainStem rdf:type owl:Class ;
				   rdfs:subClassOf nhdplusv2:FlowPath ;
				   rdfs:label "nhdplusv2:MainStem"^^xsd:string ;
				   rdfs:comment "a named river or similar feature, represented from head to outlet (a composition of elemenatry flowpaths (flowlines) per hydrologic fabric logic model)"^^xsd:string .

###  http://nhdplusv2.spatialai.org/v1/nhdplusv2#FlowPathLength
nhdplusv2:FlowPathLength rdf:type owl:Class ;
                         rdfs:subClassOf qudt:Quantity ;
						 rdfs:label "nhdplusv2:FlowPathLength"^^xsd:string ;
						 rdfs:comment "The length of a flowpath"^^xsd:string .

### HyFO ###

###  http://hyfo.spatialai.org/v1/hyfo#AquiferWaterFeature
hyfo:AquiferWaterFeature rdf:type owl:Class ;
                         rdfs:subClassOf hyfo:SubsurfaceWaterFeature ;
				         rdfs:label "hyfo:AquiferWaterFeature"^^xsd:string ;
				         rdfs:comment "An aquifer water feature including water, container, and void"^^xsd:string .

###  http://hyfo.spatialai.org/v1/hyfo#HydroRockBody
hyfo:HydroRockBody rdf:type owl:Class ;
                   rdfs:subClassOf hyfo:SubsurfaceWaterFeature ;
			       rdfs:label "hyfo:HydroRockBody"^^xsd:string ;
			       rdfs:comment "a hybrid physical object, such as aquifer, well, or lake, that consists partly of a rock body (a container), empty spaces therein (voids), and a water body inside the space"^^xsd:string ;
				   rdfs:isDefinedBy <https://www.tandfonline.com/doi/pdf/10.1080/13658816.2018.1443751> .

###  http://hyfo.spatialai.org/v1/hyfo#SubsurfaceWaterFeature
hyfo:SubsurfaceWaterFeature rdf:type owl:Class ;
						    rdfs:subClassOf hyfo:WaterFeature ;
				            rdfs:label "hyfo:SubsurfaceWaterFeature"^^xsd:string ;
				            rdfs:comment "A complete subsurface water feature including water, container, and void (for example, aquifer, well, et al.)"^^xsd:string .

###  http://hyfo.spatialai.org/v1/hyfo#SurfaceWaterFeature
hyfo:SurfaceWaterFeature rdf:type owl:Class ;
					     rdfs:subClassOf hyfo:WaterFeature ;
				         rdfs:label "hyfo:SurfaceWaterFeature"^^xsd:string ;
				         rdfs:comment "A complete surface water feature including water, container, and void (for example: lake, river, marsh, et al.)"^^xsd:string .

###  http://hyfo.spatialai.org/v1/hyfo#WaterFeature
hyfo:WaterFeature rdf:type owl:Class ;
                  rdfs:subClassOf geo:Feature ;
				  rdfs:label "hyfo:WaterFeature"^^xsd:string ;
				  rdfs:comment "A complete water feature including water, container, and void; includes surface and subsurface water features"^^xsd:string .

###  http://hyfo.spatialai.org/v1/hyfo#WaterFeatureRepresentation
hyfo:WaterFeatureRepresentation rdf:type owl:Class ;
                                rdfs:subClassOf geo:Geometry ;
				                rdfs:label "hyfo:WaterFeatureRepresentation"^^xsd:string ;
				                rdfs:comment "A realization of a water feature (for example, a line or polygon)"^^xsd:string .

###  http://hyfo.spatialai.org/v1/hyfo#WaterWell
hyfo:WaterWell rdf:type owl:Class ;
               rdfs:subClassOf hyfo:SubsurfaceWaterFeature ;
			   owl:equivalentClass gwml2:GW_Well ;
			   rdfs:label "hyfo:WaterWell"^^xsd:string ;
			   rdfs:comment "A water well, with focus on the hole/shaft itself (see gwml2:GW_Well)"^^xsd:string .

### QUDT ###

###  http://qudt.org/schema/qudt/NumericUnion
qudt:NumericUnion rdf:type owl:Class ;
                  rdfs:label "qudt:NumericUnion"^^xsd:string .

###  http://qudt.org/schema/qudt/Quantity
qudt:Quantity rdf:type owl:Class ;
			  rdfs:isDefinedBy <http://qudt.org/2.1/schema/qudt> ;
			  rdfs:label "qudt:Quantity"^^xsd:string .

###  http://qudt.org/schema/qudt/QuantityKind
qudt:QuantityKind rdf:type owl:Class ;
			      rdfs:isDefinedBy <http://qudt.org/2.1/schema/qudt> ;
			      rdfs:label "qudt:QuantityKind"^^xsd:string .

###  http://qudt.org/schema/qudt/QuantityValue
qudt:QuantityValue rdf:type owl:Class ;
				   rdfs:isDefinedBy <http://qudt.org/2.1/schema/qudt> ;
				   rdfs:label "qudt:QuantityValue"^^xsd:string.

###  http://qudt.org/schema/qudt/Unit
qudt:Unit rdf:type owl:Class ;
		  rdfs:isDefinedBy <http://qudt.org/2.1/schema/qudt> ;
		  rdfs:label "qudt:Unit"^^xsd:string.


#################################################################
#    General Axioms
#################################################################

[ rdf:type owl:AllDisjointClasses ;
  owl:members ( hyf:HY_Canal
                hyf:HY_Estuary
				hyf:HY_Impoundment
				hyf:HY_Lagoon
				hyf:HY_Lake
                hyf:HY_River
			  )
] .

[ rdf:type owl:AllDisjointClasses ;
  owl:members ( hyf:HY_CatchmentArea
				hyf:HY_CatchmentDivide
			  )
] .

[ rdf:type owl:AllDisjointClasses ;
  owl:members ( hyf:HY_CatchmentRealization
                hyf:HY_HydroFeature
			  )
] .

[ rdf:type owl:AllDisjointClasses ;
  owl:members ( hyfo:AquiferWaterFeature
                hyfo:WaterWell
			  )
] .

[ rdf:type owl:AllDisjointClasses ;
  owl:members ( hyfo:SubsurfaceWaterFeature
                hyfo:SurfaceWaterFeature
			  )
] .

[ rdf:type owl:AllDisjointClasses ;
  owl:members ( hyfo:WaterFeature
				hyfo:WaterFeatureRepresentation
			  )
] .


#################################################################
#    Individuals
#################################################################


